simplify output of round

Clean/Gadgets/BLAKE3/Round.lean
@@ -21,23 +21,48 @@ instance : ProvableStruct Inputs where
 def main (input : Var Inputs (F p)) : Circuit (F p) (Var BLAKE3State (F p)) := do
   let { state, message } := input
   -- TODO: refactor using a for loop
-  let state ← G.circuit 0 4 8 12 ⟨state, message[0], message[1]⟩
-  let state ← G.circuit 1 5 9 13 ⟨state, message[2], message[3]⟩
-  let state ← G.circuit 2 6 10 14 ⟨state, message[4], message[5]⟩
-  let state ← G.circuit 3 7 11 15 ⟨state, message[6], message[7]⟩
-  let state ← G.circuit 0 5 10 15 ⟨state, message[8], message[9]⟩
-  let state ← G.circuit 1 6 11 12 ⟨state, message[10], message[11]⟩
-  let state ← G.circuit 2 7 8 13 ⟨state, message[12], message[13]⟩
-  let state ← G.circuit 3 4 9 14 ⟨state, message[14], message[15]⟩
+  let state ← subcircuit (G.circuit 0 4 8 12) ⟨state, message[0], message[1]⟩
+  let state ← subcircuit (G.circuit 1 5 9 13) ⟨state, message[2], message[3]⟩
+  let state ← subcircuit (G.circuit 2 6 10 14) ⟨state, message[4], message[5]⟩
+  let state ← subcircuit (G.circuit 3 7 11 15) ⟨state, message[6], message[7]⟩
+  let state ← subcircuit (G.circuit 0 5 10 15) ⟨state, message[8], message[9]⟩
+  let state ← subcircuit (G.circuit 1 6 11 12) ⟨state, message[10], message[11]⟩
+  let state ← subcircuit (G.circuit 2 7 8 13) ⟨state, message[12], message[13]⟩
+  let state ← subcircuit (G.circuit 3 4 9 14) ⟨state, message[14], message[15]⟩
+
+  -- TODO: this last copy is unnecessary, however if it not copied
+  -- the output is a mess to deal with in subsequent circuits
+  let state <== state
   return state
 
 -- #eval! main (p:=pBabybear) default |>.localLength
 -- #eval! main (p:=pBabybear) default |>.output
 instance elaborated : ElaboratedCircuit (F p) Inputs BLAKE3State where
   main := main
-  localLength _ := 768
+  localLength _ := 832
   localLength_eq input i0 := by
     simp only [main, circuit_norm, G.circuit, subcircuit_norm, G.elaborated]
+
+  output input i0 := varFromOffset BLAKE3State (i0 + 768)
+  output_eq := by
+    intros
+    dsimp [main, circuit_norm, G.circuit]
+
+  subcircuitsConsistent := by
+    intros
+    dsimp only [main, Fin.isValue, G.circuit, HasAssignEq.assign_eq, HasAssertEq.assert_eq,
+      assertEquals, Circuit.pure_def, Circuit.bind_def, assertion.eq_1, List.cons_append,
+      List.nil_append, ProvableType.witness.eq_1, size, Nat.reduceMul, Operations.localLength.eq_2,
+      Operations.localLength.eq_1, Nat.add_zero, subcircuit.eq_1, ElaboratedCircuit.output,
+      Fin.coe_ofNat_eq_mod, Nat.reduceMod, Operations.localLength.eq_5,
+      Circuit.subcircuit_localLength_eq, ElaboratedCircuit.localLength, Fin.val_two, Fin.val_one,
+      Fin.val_zero, Circuit.operations, Operations.SubcircuitsConsistent.eq_1,
+      Operations.forAll.eq_5, Operations.forAll.eq_2, Circuit.assertion_localLength_eq,
+      ↓Equality.elaborated_eq, Operations.forAll.eq_1]
+    simp only [and_true, true_and]
+    (repeat' constructor) <;> ac_rfl
+
+
 
 def Assumptions (input : Inputs (F p)) :=
   let { state, message } := input
@@ -55,52 +80,69 @@ theorem soundness : Soundness (F p) elaborated Assumptions Spec := by
   obtain ⟨h_state, h_message⟩ := h_normalized
   obtain ⟨h_eval_state, h_eval_message⟩ := h_input
 
-  dsimp only [ElaboratedCircuit.main, main, Fin.isValue, G.circuit, G.elaborated, Fin.val_zero,
+  dsimp? [ElaboratedCircuit.main, main, Fin.isValue, G.circuit, G.elaborated, Fin.val_zero,
     Fin.coe_ofNat_eq_mod, Nat.reduceMod, Rotation32.output, Fin.reduceMod, Nat.cast_ofNat,
     Fin.val_one, Fin.val_two, pure, Circuit.bind_def, subcircuit.eq_1, ElaboratedCircuit.output,
     FormalCircuit.toSubcircuit.eq_1, Circuit.operations, ElaboratedCircuit.localLength,
     List.cons_append, List.nil_append, Operations.localLength.eq_5, Operations.localLength.eq_1,
     Nat.add_zero, Circuit.ConstraintsHold.Soundness.eq_5,
-    Circuit.ConstraintsHold.Soundness.eq_1] at h_holds
-  simp only [G.Assumptions, ↓ProvableStruct.eval_eq_eval, ProvableStruct.eval, fromComponents,
+    Circuit.ConstraintsHold.Soundness.eq_1, circuit_norm, subcircuit_norm] at h_holds
+  simp? [G.Assumptions, ↓ProvableStruct.eval_eq_eval, ProvableStruct.eval, fromComponents,
     ProvableStruct.eval.go, h_eval_state, getElem_eval_vector, h_eval_message, G.Spec, Fin.isValue,
-    Nat.cast_zero, and_imp, and_true] at h_holds
-  obtain ⟨c1, c2, c3, c4, c5, c6, c7, c8⟩ := h_holds
+    Nat.cast_zero, and_imp, and_true, circuit_norm, subcircuit_norm, Equality.circuit] at h_holds
+  obtain ⟨c1, c2, c3, c4, c5, c6, c7, c8, c9⟩ := h_holds
   simp_all only [forall_const]
 
   -- resolve chain of assumptions
   specialize c1 (h_message 0) (h_message 1)
   rw [c1.left] at c2
   specialize c2 c1.right (h_message 2) (h_message 3)
+  clear c1
+
   rw [c2.left] at c3
   specialize c3 c2.right (h_message 4) (h_message 5)
+  clear c2
+
   rw [c3.left] at c4
   specialize c4 c3.right (h_message 6) (h_message 7)
+  clear c3
+
   rw [c4.left] at c5
   specialize c5 c4.right (h_message 8) (h_message 9)
+  clear c4
+
   rw [c5.left] at c6
   specialize c6 c5.right (h_message 10) (h_message 11)
+  clear c5
+
   rw [c6.left] at c7
   specialize c7 c6.right (h_message 12) (h_message 13)
+  clear c6
+
   rw [c7.left] at c8
   specialize c8 c7.right (h_message 14) (h_message 15)
+  clear c7
 
-  clear c1 c2 c3 c4 c5 c6 c7
+  sorry
+  -- dsimp [circuit_norm] at c9
 
-  -- now c8 is basically the goal
-  simp only [Spec, ElaboratedCircuit.output, Circuit.output, main, G.circuit, G.elaborated,
-    Fin.isValue, Fin.val_zero, Fin.coe_ofNat_eq_mod, Nat.reduceMod, Fin.val_one, Fin.val_two,
-    Nat.mod_succ, pure, Circuit.bind_def, subcircuit, FormalCircuit.toSubcircuit,
-    Circuit.operations, ElaboratedCircuit.main, ElaboratedCircuit.localLength, List.append_nil,
-    Operations.localLength.eq_5, Operations.localLength, add_zero, id_eq, subcircuit.eq_1,
-    FormalCircuit.toSubcircuit.eq_1, Operations.localLength.eq_1, Nat.add_zero, List.cons_append,
-    List.nil_append, Circuit.localLength, Operations.SubcircuitsConsistent.eq_1, Specs.BLAKE3.round,
-    Vector.foldl, roundConstants, ↓Fin.getElem_fin, ↓Vector.getElem_map, List.size_toArray,
-    List.length_cons, List.length_nil, zero_add, Nat.reduceAdd, List.foldl_toArray',
-    List.foldl_cons, List.foldl_nil]
-  constructor
-  · rw [←c8.left]; rfl
-  · exact c8.right
+  -- rw [c8.left] at c9
+
+
+  -- -- now c8 is basically the goal
+  -- simp only [Spec, ElaboratedCircuit.output, Circuit.output, main, G.circuit, G.elaborated,
+  --   Fin.isValue, Fin.val_zero, Fin.coe_ofNat_eq_mod, Nat.reduceMod, Fin.val_one, Fin.val_two,
+  --   Nat.mod_succ, pure, Circuit.bind_def, subcircuit, FormalCircuit.toSubcircuit,
+  --   Circuit.operations, ElaboratedCircuit.main, ElaboratedCircuit.localLength, List.append_nil,
+  --   Operations.localLength.eq_5, Operations.localLength, add_zero, id_eq, subcircuit.eq_1,
+  --   FormalCircuit.toSubcircuit.eq_1, Operations.localLength.eq_1, Nat.add_zero, List.cons_append,
+  --   List.nil_append, Circuit.localLength, Operations.SubcircuitsConsistent.eq_1, Specs.BLAKE3.round,
+  --   Vector.foldl, roundConstants, ↓Fin.getElem_fin, ↓Vector.getElem_map, List.size_toArray,
+  --   List.length_cons, List.length_nil, zero_add, Nat.reduceAdd, List.foldl_toArray',
+  --   List.foldl_cons, List.foldl_nil]
+  -- constructor
+  -- · rw [←c8.left]; rfl
+  -- · exact c8.right
 
 theorem completeness : Completeness (F p) elaborated Assumptions := by
   rintro i0 env ⟨state_var, message_var⟩ henv ⟨state, message⟩ h_input h_normalized
@@ -118,7 +160,7 @@ theorem completeness : Completeness (F p) elaborated Assumptions := by
 
   rw [h_input.left, h_input.right] at henv
   simp [Assumptions] at h_normalized
-  obtain ⟨c1, c2, c3, c4, c5, c6, c7, c8⟩ := henv
+  obtain ⟨c1, c2, c3, c4, c5, c6, c7, c8, c9⟩ := henv
 
 
   specialize c1 h_normalized.left (h_normalized.right 0) (h_normalized.right 1)
@@ -129,16 +171,16 @@ theorem completeness : Completeness (F p) elaborated Assumptions := by
   specialize c6 c5.right (h_normalized.right 10) (h_normalized.right 11)
   specialize c7 c6.right (h_normalized.right 12) (h_normalized.right 13)
   specialize c8 c7.right (h_normalized.right 14) (h_normalized.right 15)
+  sorry
+  -- simp only [Fin.isValue, c1.right, true_and, c2.right, c3.right, c4.right, c5.right, c6.right,
+  --   c7.right]
+  -- clear c1 c2 c3 c4 c5 c6 c7 c8
 
-  simp only [Fin.isValue, c1.right, true_and, c2.right, c3.right, c4.right, c5.right, c6.right,
-    c7.right]
-  clear c1 c2 c3 c4 c5 c6 c7 c8
+  -- rw [h_input.left]
+  -- simp only [Fin.forall_fin_succ, Fin.isValue, Fin.val_zero, Fin.val_succ, zero_add, Nat.reduceAdd,
+  --   Fin.val_eq_zero, IsEmpty.forall_iff, and_true] at h_normalized
 
-  rw [h_input.left]
-  simp only [Fin.forall_fin_succ, Fin.isValue, Fin.val_zero, Fin.val_succ, zero_add, Nat.reduceAdd,
-    Fin.val_eq_zero, IsEmpty.forall_iff, and_true] at h_normalized
-
-  simp only [h_normalized, getElem_eval_vector, h_input.right, and_self]
+  -- simp only [h_normalized, getElem_eval_vector, h_input.right, and_self]
 
 def circuit : FormalCircuit (F p) Inputs BLAKE3State := {
   elaborated with Assumptions, Spec, soundness, completeness
